src/mulx/CorrectnessProof.ec
@@ -1,10 +1,13 @@
-require import AllCore Bool List Int IntDiv StdOrder CoreMap Real Zp_25519 Ring Distr.
+require import AllCore Bool List Int IntDiv StdOrder CoreMap Real Ring Distr.
 
 from Jasmin require import JModel JMemory JWord.
 
-require import Curve25519_Procedures Curve25519_auto_mulx Curve25519_mulx W64limbs Zp_25519 Zplimbs EClib.
+require import Curve25519_Procedures Curve25519_Operations Curve25519_auto_mulx Curve25519_mulx W64limbs Zp_25519 Zplimbs EClib.
 
-import Zp Curve25519_auto_mulx Curve25519_Procedures Curve25519_mulx Array4 Array8 Array32 StdOrder.IntOrder EClib.
+import Zp Curve25519_auto_mulx Curve25519_Operations Curve25519_Procedures Curve25519_mulx Array4 Array8 Array32 StdOrder.IntOrder EClib.
+
+
+abbrev zexp = ZModpRing.exp.
 
 (* additions, substractions and powers *)
 equiv eq_spec_impl_add_sss_mulx : CurveProcedures.add ~ M_mulx.__add4_sss:
@@ -324,51 +327,313 @@ proof.
         call eq_spec_impl_montgomery_ladder_step_mulx. wp. call eq_spec_impl_init_points_mulx. skip. done.
 qed.
 
+
 (** step 9 : invert **)
-lemma eq_spec_impl__it_sqr_mulx (i1: int) (i2: int):
-i1 = 2*i2 => 0 < i1 =>
-   equiv[
-        CurveProcedures.it_sqr ~ M_mulx.__it_sqr4_x2:
-        i1 = i{1} /\
-        i2 = to_uint i{2} /\
-        f{1} = inzpRep4 f{2}
+
+equiv eq_spec_impl_it_sqr_aux_mulx :
+        M_mulx.__it_sqr4_x2 ~ CurveProcedures.it_sqr_aux:
+        inzpRep4 f{1} = a{2} /\
+        W32.to_uint i{1} = l{2} /\
+        0 < l{2}
         ==>
-        res{1} = inzpRep4 res{2}].
+        inzpRep4 res{1} = res{2}.
 proof.
-    move => H H0.
-    proc. admit. (* for manuel *)
+    proc; simplify.
+    while(
+        0 <= ii{2} /\ 0 <= W32.to_uint i{1} /\ ii{2} = W32.to_uint i{1} /\
+        f{2} = inzpRep4 f{1}  /\ zf{1} = (0 = W32.to_uint i{1})
+    ).
+    wp.
+    symmetry.
+    call eq_spec_impl__sqr_rr_mulx. call eq_spec_impl__sqr_rr_mulx. wp. symmetry.
+    skip => />.
+    move => &1 *. do split. smt().
+    rewrite /DEC_32 /rflags_of_aluop_nocf_w => />.
+    + rewrite to_uintB. rewrite uleE to_uint1; smt(). rewrite to_uint1. smt(W32.to_uint_cmp).
+    rewrite /DEC_32 /rflags_of_aluop_nocf_w => />. rewrite to_uintB.
+    + rewrite uleE to_uint1; smt(). rewrite to_uint1 //.
+    rewrite /DEC_32 /rflags_of_aluop_nocf_w => />. rewrite /ZF_of to_uintB.
+    + rewrite uleE to_uint1. smt(). rewrite -to_uintB. rewrite uleE. smt(W32.to_uint_cmp).
+    + rewrite to_uintB. rewrite uleE to_uint1; smt(). rewrite to_uint1.
+    smt(W32.ge2_modulus W32.of_uintK W32.to_uintK W32.of_intD).
+    rewrite /DEC_32 /rflags_of_aluop_nocf_w => />. rewrite /ZF_of => *.
+    smt(W32.ge2_modulus W32.of_uintK W32.to_uintK W32.to_uintN W32.of_intD).
+    rewrite /DEC_32 /rflags_of_aluop_nocf_w => />. rewrite /ZF_of => *.
+    smt(W32.ge2_modulus W32.of_uintK W32.to_uintK W32.to_uintN W32.of_intD).
+    wp. call eq_spec_impl__sqr_rr_mulx_rev. call eq_spec_impl__sqr_rr_mulx_rev. wp.
+    skip => />. move => &1 H.
+    do split. smt().
+    rewrite /DEC_32 /rflags_of_aluop_nocf_w => />. rewrite /ZF_of => *.
+    smt(W32.ge2_modulus W32.of_uintK W32.to_uintK W32.to_uintN W32.of_intD).
+    rewrite /DEC_32 /rflags_of_aluop_nocf_w => />. rewrite /ZF_of => *.
+    rewrite to_uintB. rewrite uleE to_uint1. smt(W32.to_uint_cmp). rewrite to_uint1 //.
+    rewrite /DEC_32 /rflags_of_aluop_nocf_w => />. rewrite /ZF_of => *.
+    smt(W32.ge2_modulus W32.of_uintK W32.to_uintK W32.to_uintN W32.of_intD).
+    rewrite /DEC_32 /rflags_of_aluop_nocf_w => />. rewrite /ZF_of => *.
+    smt(W32.ge2_modulus W32.of_uintK W32.to_uintK W32.to_uintN W32.of_intD).
+    rewrite /DEC_32 /rflags_of_aluop_nocf_w => />. rewrite /ZF_of => *.
+    smt(W32.ge2_modulus W32.of_uintK W32.to_uintK W32.to_uintN W32.of_intD).
 qed.
+
+equiv eq_spec_impl_it_sqr_aux_mulx_test :
+        CurveProcedures.it_sqr_aux ~ M_mulx.__it_sqr4_x2:
+        a{1} = inzpRep4 f{2} /\
+        l{1} = W32.to_uint i{2} /\
+        0 < l{1}
+        ==>
+        res{1} = inzpRep4 res{2}.
+proof.
+    proc; simplify.
+    while(
+        0 <= ii{1} /\ 0 <= W32.to_uint i{2} /\ ii{1} = W32.to_uint i{2} /\
+        f{1} = inzpRep4 f{2}  /\ zf{2} = (0 = W32.to_uint i{2})
+    ).
+    wp. call eq_spec_impl__sqr_rr_mulx. call eq_spec_impl__sqr_rr_mulx. wp.
+    skip => />.
+    move => &1 *. do split. smt().
+    rewrite /DEC_32 /rflags_of_aluop_nocf_w => />.
+    + rewrite to_uintB. rewrite uleE to_uint1; smt(). rewrite to_uint1. smt(W32.to_uint_cmp).
+    rewrite /DEC_32 /rflags_of_aluop_nocf_w => />. rewrite to_uintB.
+    + rewrite uleE to_uint1; smt(). rewrite to_uint1 //.
+    rewrite /DEC_32 /rflags_of_aluop_nocf_w => />. rewrite /ZF_of to_uintB.
+    + rewrite uleE to_uint1. smt(). rewrite -to_uintB. rewrite uleE. smt(W32.to_uint_cmp).
+    + rewrite to_uintB. rewrite uleE to_uint1; smt(). rewrite to_uint1.
+    smt(W32.ge2_modulus W32.of_uintK W32.to_uintK W32.of_intD).
+    rewrite /DEC_32 /rflags_of_aluop_nocf_w => />. rewrite /ZF_of => *.
+    smt(W32.ge2_modulus W32.of_uintK W32.to_uintK W32.to_uintN W32.of_intD).
+    rewrite /DEC_32 /rflags_of_aluop_nocf_w => />. rewrite /ZF_of => *.
+    smt(W32.ge2_modulus W32.of_uintK W32.to_uintK W32.to_uintN W32.of_intD).
+    wp. call eq_spec_impl__sqr_rr_mulx. call eq_spec_impl__sqr_rr_mulx. wp.
+    skip => />. move => &1 H.
+    do split. smt().
+    rewrite /DEC_32 /rflags_of_aluop_nocf_w => />. rewrite /ZF_of => *.
+    smt(W32.ge2_modulus W32.of_uintK W32.to_uintK W32.to_uintN W32.of_intD).
+    rewrite /DEC_32 /rflags_of_aluop_nocf_w => />. rewrite /ZF_of => *.
+    rewrite to_uintB. rewrite uleE to_uint1. smt(W32.to_uint_cmp). rewrite to_uint1 //.
+    rewrite /DEC_32 /rflags_of_aluop_nocf_w => />. rewrite /ZF_of => *.
+    smt(W32.ge2_modulus W32.of_uintK W32.to_uintK W32.to_uintN W32.of_intD).
+    rewrite /DEC_32 /rflags_of_aluop_nocf_w => />. rewrite /ZF_of => *.
+    smt(W32.ge2_modulus W32.of_uintK W32.to_uintK W32.to_uintN W32.of_intD).
+    rewrite /DEC_32 /rflags_of_aluop_nocf_w => />. rewrite /ZF_of => *.
+    smt(W32.ge2_modulus W32.of_uintK W32.to_uintK W32.to_uintN W32.of_intD).
+qed.
+
+
+lemma eq_spec_impl__it_sqr_mulx (i1: int) (i2: int):
+    i1 = i2 => 2 <= i1  =>
+equiv[
+        M_mulx.__it_sqr4_x2 ~ CurveProcedures.it_sqr:
+        i1 = W32.to_uint i{1} /\
+        i2 = i{2}   /\
+        W32.to_uint i{1} = i{2} /\
+        inzpRep4 f{1} = f{2}
+        ==>
+        inzpRep4 res{1} = zexp res{2} (exp 2 i1)
+    ].
+proof.
+    move => I I0.
+    transitivity
+     CurveProcedures.it_sqr_aux
+     (
+       l{2} = W32.to_uint i{1}  /\
+       a{2} = inzpRep4 f{1} /\
+       1 < l{2}
+        ==>
+        inzpRep4 res{1} = res{2})
+     (  a{1} = f{2} /\
+        l{1} = i{2} /\
+        l{1} = i1 /\
+        l{1} = i2 /\
+        2 <= i{2}
+        ==>
+        res{1} = zexp res{2} (exp 2 i1)).
+    auto => />.
+    move => &1 &2 *.
+    exists(f{2}, i{2}) => />. smt().
+    move => &1 &m &2 H H0. rewrite -H0. assumption.
+    proc *.
+    call eq_spec_impl_it_sqr_aux_mulx. skip => />. smt(W32.to_uint_cmp).
+
+    proc; inline *; simplify.
+    seq 7 6 : (ii{1} = l{1} - 1 /\
+        h{2} = (zexp a{1} 2) /\
+        0 <= ii{2} /\
+        0 <= ii{1} /\
+        ii{1} = ii{2} /\
+        1 <= counter{2} <= i1 /\
+        counter{2} = i1 - ii{2} /\
+        f{1} = zexp h{2} (exp 2 counter{2})).
+        wp; skip. auto => />. move => *.  smt().
+
+    while(
+        0 <= ii{1} /\
+        0 <= ii{2} /\
+        ii{1} = ii{2} /\
+        1 <= counter{2} /\
+        counter{2} = i1 - ii{2} /\
+        f{1} = zexp h{2} (exp 2 (counter{2}))).
+    wp; skip. auto => />.
+    move => &1 &2 H H0 H1.
+    smt( ZModpRing.exprM IntID.exprN IntID.exprN1 IntID.exprD_nneg).
+    skip => />. move => &1 &2 H H1 H2 H3 H4 H5 H6 H7 H8 H9.
+    have H10: H4 = 0. smt(). rewrite H10 => />.
+qed.
+
+lemma eq_spec_impl__it_sqr_mulx_x2 (i1: int) (i2: int):
+    2*i1 = i2 => 2 <= i1 => 4 <= i2 => i2 %% 2 = 0 =>
+equiv[
+        M_mulx.__it_sqr4_x2 ~ CurveProcedures.it_sqr:
+        i1 = W32.to_uint i{1} /\
+        i2 = i{2}   /\
+        2*W32.to_uint i{1} = i{2} /\
+        i{2} %% 2 = 0 /\
+        inzpRep4 f{1} = f{2}
+        ==>
+        inzpRep4 res{1} = res{2}
+    ].
+proof.
+    move => I I0 I1 I2;
+     transitivity
+     CurveProcedures.it_sqr_aux
+     (
+       l{2} = W32.to_uint i{1}  /\
+       a{2} = inzpRep4 f{1} /\
+       1 < l{2}
+        ==>
+        inzpRep4 res{1} = res{2})
+     (  a{1} = f{2} /\
+        2*l{1} = i{2} /\
+        l{1} = i1 /\
+        i{2} = i2  /\
+        4 <= i{2}  /\
+        2 <= l{1}
+        ==>
+        res{1} = res{2}).
+    auto => />. move => &1 &2 *.
+    exists(f{2}, i1) => />. smt(). smt().
+    proc *.
+    call eq_spec_impl_it_sqr_aux_mulx. skip => />. smt(W32.to_uint_cmp).
+     proc; simplify. inline *.
+     seq 7 6 : (
+        i2 = 2*l{1} /\
+        ii{1} = l{1} - counter{2} /\
+        ii{2} = i2 - counter{2} /\
+        h{2} = (zexp a{1} 2) /\
+        0 <= ii{2} /\
+        0 <= ii{1} /\
+        1 <= counter{2} <= i1 /\
+        f{1} = zexp h{2} (exp 2 counter{2})).
+    wp; skip. auto => />.
+    move => *. smt().
+      async while
+      [ (fun r => 0%r < ii%r), (ii{1} - 1)%r ]
+      [ (fun r => 0%r < ii%r), (ii{1} - 1)%r ]
+        (0 < ii{1} /\ 0 < ii{2}) (!(0 < ii{1}))
+      :
+      (
+        (ii{2} %% 2 = 0   => 2*ii{1} - 1 = ii{2})  /\
+        (ii{2} %% 2 <> 0  => 2*ii{1}     = ii{2})  /\
+        0 <= ii{1} /\
+        0 <= ii{2}
+      ).
+    auto => />;  move => &1 &2 * /#.
+    auto => />;  move => &1 &2 * /#.
+    auto => />;  move => &1 &2 * /#.
+    auto => />;  move => &2 * /#.
+    move => &1; auto => />.
+    move => v1 v2; auto => />.
+    while(
+        0 <= ii{1} /\
+        0 <= ii{2} /\
+        (ii{2} %% 2 = 0   => 2*ii{1} - 1 = ii{2})  /\
+        (ii{2} %% 2 <> 0  => 2*ii{1}     = ii{2})  /\
+        1 <= counter{2} /\
+        f{1} = zexp h{2} (exp 2 counter{2})
+    ) => //=.
+   auto => />; move => &1 &2 H H0 H1 H2 H3 H4 H5 H6 H7.
+   smt( ZModpRing.exprM IntID.exprN IntID.exprN1 IntID.exprD_nneg).
+   auto => />; move => &1 &2 H H0 H1 H2 H3 H4 H5.
+   smt( ZModpRing.exprM IntID.exprN IntID.exprN1 IntID.exprD_nneg).
+    while true (ii) => //.
+    move => H; auto => />. skip => />; move => &hr H0 H1 H2 H3 H4 H5 /#.
+    while true (ii) => //. move => H; auto => /> /#. skip => /> /#.
+    skip => />. move => &1 &2 H H0 H1 H2 H3 H4 H5 H6 H7 H8 H9 H10 H11 H12 H13 /#.
+qed.
+
 
 lemma eq_spec_impl_it_sqr_x2_mulx (i1: int) (i2: int):
-    i1 = 2*i2 => 0 < i1 =>
-    equiv [CurveProcedures.it_sqr ~ M_mulx._it_sqr4_x2:
-        i1 = i{1} /\
-        i2 = to_uint i{2} /\
-        f{1} = inzpRep4 f{2}
-         ==>
-        res{1} = inzpRep4 res{2}].
-proof.
-   move => H H0.
-   proc *. simplify. inline {2} 1.
-   wp. sp. call (eq_spec_impl__it_sqr_mulx i1 i2).
-   skip. done.
+    i1 = i2 => 2 <= i1 => i2 %% 2 = 0 =>
+equiv[
+        M_mulx._it_sqr4_x2 ~ CurveProcedures.it_sqr:
+        i1 = W32.to_uint i{1} /\
+        i2 = i{2}   /\
+        W32.to_uint i{1} = i{2} /\
+        i{2} %% 2 = 0 /\
+        inzpRep4 f{1} = f{2}
+        ==>
+        inzpRep4 res{1} = zexp res{2} (exp 2 i1)
+    ].
+    move => *; proc *.
+    inline {1} 1. sp; wp.
+    call (eq_spec_impl__it_sqr_mulx i1 i2). skip => />.
 qed.
 
-lemma eq_spec_impl_it_sqr_x2__mulx (i1: int) (i2: int):
-    i1 = 2*i2 => 0 < i1 =>
-    equiv [CurveProcedures.it_sqr ~ M_mulx._it_sqr4_x2_:
-        i1 = i{1} /\
-        i2 = to_uint i{2} /\
-        f{1} = inzpRep4 _f{2}
-         ==>
-        res{1} = inzpRep4 res{2}].
+
+lemma  eq_spec_impl_it_sqr_x2__mulx  (i1: int) (i2: int):
+    i1 = i2 => 2 <= i1 => i2 %% 2 = 0 =>
+    equiv[
+        M_mulx._it_sqr4_x2_ ~ CurveProcedures.it_sqr:
+        i1 = W32.to_uint i{1} /\
+        i2 = i{2}   /\
+        W32.to_uint i{1} = i{2} /\
+        i{2} %% 2 = 0 /\
+        inzpRep4 _f{1} = f{2}
+        ==>
+        inzpRep4 res{1} = zexp res{2} (exp 2 i1)
+    ].
 proof.
-    move => H H0.
-    proc *. simplify.
-    inline{2} 1. wp. sp.
-    call (eq_spec_impl_it_sqr_x2_mulx i1 i2).
-    skip. done.
+    move => *; proc *.
+    inline{1} 1. inline{1} 5. wp; sp.
+    call (eq_spec_impl__it_sqr_mulx i1 i2). skip => />.
 qed.
+
+
+lemma eq_spec_impl_it_sqr_x2_mulx_x2 (i1: int) (i2: int):
+    2*i1 = i2 => 2 <= i1 => 4 <= i2 => i2 %% 2 = 0 =>
+equiv[
+        M_mulx._it_sqr4_x2 ~ CurveProcedures.it_sqr:
+       i1 = W32.to_uint i{1} /\
+        i2 = i{2}   /\
+        2*W32.to_uint i{1} = i{2} /\
+        i{2} %% 2 = 0 /\
+        inzpRep4 f{1} = f{2}
+        ==>
+        inzpRep4 res{1} = res{2}
+    ].
+    move => *; proc *.
+    inline {1} 1. sp; wp.
+    call (eq_spec_impl__it_sqr_mulx_x2 i1 i2). skip => />.
+qed.
+
+
+lemma  eq_spec_impl_it_sqr_x2__mulx_x2  (i1: int) (i2: int):
+    2*i1 = i2 => 2 <= i1 => 4 <= i2 => i2 %% 2 = 0 =>
+        equiv[
+        M_mulx._it_sqr4_x2_ ~ CurveProcedures.it_sqr:
+         i1 = W32.to_uint i{1} /\
+        i2 = i{2}   /\
+        2*W32.to_uint i{1} = i{2} /\
+        i{2} %% 2 = 0 /\
+        inzpRep4 _f{1} = f{2}
+        ==>
+        inzpRep4 res{1} = res{2}
+    ].
+proof.
+    move => *; proc *.
+    inline{1} 1. inline{1} 5. wp; sp.
+    call (eq_spec_impl__it_sqr_mulx_x2 i1 i2). skip => />.
+qed.
+
 
 
 lemma eq_spec_impl_invert_mulx (i1: int) (i2: int) :
@@ -384,21 +649,21 @@ proof.
     auto => />.
     call eq_spec_impl_mul_rsr__mulx.
     call eq_spec_impl_sqr_rr__mulx.
-    call (eq_spec_impl_it_sqr_x2__mulx 4 2). wp.
+    symmetry;  call (eq_spec_impl_it_sqr_x2__mulx_x2 2 4); wp; symmetry.
     call eq_spec_impl_mul_rsr__mulx.
-    call (eq_spec_impl_it_sqr_x2__mulx 50 25). wp.
+    symmetry;  call (eq_spec_impl_it_sqr_x2__mulx_x2 25 50); wp; symmetry.
     call eq_spec_impl_mul_rsr__mulx.
-    call (eq_spec_impl_it_sqr_x2__mulx 100 50). wp.
+    symmetry;  call (eq_spec_impl_it_sqr_x2__mulx_x2 50 100); wp; symmetry.
     call eq_spec_impl_mul_rsr__mulx.
-    call (eq_spec_impl_it_sqr_x2__mulx 50 25). wp.
+    symmetry;  call (eq_spec_impl_it_sqr_x2__mulx_x2 25 50); wp; symmetry.
     call eq_spec_impl_mul_rsr__mulx.
-    call (eq_spec_impl_it_sqr_x2__mulx 10 5). wp.
+    symmetry;  call (eq_spec_impl_it_sqr_x2__mulx_x2 5 10); wp; symmetry.
     call eq_spec_impl_mul_rsr__mulx.
-    call (eq_spec_impl_it_sqr_x2__mulx 20 10). wp.
+    symmetry;  call (eq_spec_impl_it_sqr_x2__mulx_x2 10 20); wp; symmetry.
     call eq_spec_impl_mul_rsr__mulx.
-    call (eq_spec_impl_it_sqr_x2__mulx 10 5). wp.
+    symmetry;  call (eq_spec_impl_it_sqr_x2__mulx_x2 5 10); wp; symmetry.
     call eq_spec_impl_mul_rsr__mulx. wp.
-    call (eq_spec_impl_it_sqr_x2__mulx 4 2). wp.
+    symmetry;  call (eq_spec_impl_it_sqr_x2__mulx_x2 2 4); wp; symmetry.
     call eq_spec_impl_sqr_rr__mulx. wp.
     call eq_spec_impl_mul_rsr__mulx.
     call eq_spec_impl_sqr_rr__mulx. wp.
